Improved reasoning about explode, xor gates

src/cnf/clause.lean
@@ -36,18 +36,13 @@ instance has_decidable_eq [s : decidable_eq literal] : decidable_eq clause
   end
 
 instance : has_mem literal clause := ⟨list.mem⟩
-
 instance : has_emptyc clause := ⟨list.nil⟩
-
 instance : has_union clause := ⟨list.union⟩
-
 instance : has_inter clause := ⟨list.inter⟩
-
 instance : has_singleton literal clause := ⟨λ l, [l]⟩ 
-
 instance : has_insert literal clause := ⟨list.insert⟩
-
 instance : has_append clause := ⟨list.append⟩
+instance : has_subset clause := ⟨list.subset⟩
 
 /- The clause represents a disjunction, so we evaluate literals until tt is found -/
 def eval (α : assignment) (c : clause) : bool :=
@@ -55,10 +50,11 @@ def eval (α : assignment) (c : clause) : bool :=
 
 @[simp] theorem eval_nil (α : assignment) : eval α [] = ff := rfl
 
-@[simp] theorem eval_singleton (α : assignment) (l : literal) : eval α [l] = literal.eval α l := by simp [eval]
+@[simp] theorem eval_singleton (α : assignment) (l : literal) : eval α [l] = literal.eval α l :=
+by simp [eval]
 
 theorem eval_cons (α : assignment) (l : literal) (c : clause) : eval α (l :: c) = (literal.eval α l) || (eval α c) :=
-  by simp [eval, bool.bor_comm]
+by simp [eval, bool.bor_comm]
 
 theorem eval_erase_of_mem (α : assignment) {l : literal} {c : clause} (h : l ∈ c) : eval α c = (literal.eval α l) || (eval α (c.erase l)) :=
 begin
@@ -70,12 +66,12 @@ begin
 end
 
 theorem eval_erase_of_not_mem {α : assignment} {l : literal} {c : clause} (h : l ∉ c) : eval α c = eval α (c.erase l) :=
-  by simp [erase_of_not_mem h]
+by simp [erase_of_not_mem h]
 
 /-! ### Similarity of clauses -/
 -- Because clauses are literals joined by ORs, and OR is commutative, similar clauses evaluate identically
 
-theorem eval_sim {α : assignment} {c₁ : clause} : ∀ (c₂ : clause), c₁ ~ c₂ → eval α c₁ = eval α c₂ :=
+theorem eval_sim (α : assignment) {c₁ : clause} : ∀ (c₂ : clause), c₁ ~ c₂ → eval α c₁ = eval α c₂ :=
 begin
   induction c₁ with l c ih; intros c₂ h,
   { simp [perm.nil_eq h] },
@@ -86,9 +82,9 @@ end
 -- A potentially helpful lemma stating that if a clause mapped to vars is similar to a list,
 -- then for any nat, there is a literal whose variable is that nat
 -- NOTE: Another version of this can be proven with no duplicates in either the clause or the list, via ↔
-lemma all_mem_of_sim_var {ns : list nat} : ∀ (c : clause), length c = length ns → c.map var ~ ns → ∀ n ∈ ns, ∃ l ∈ c, literal.var l = n :=
+lemma all_mem_of_sim_var {ns : list nat} : ∀ (c : clause), c.map var ~ ns → ∀ n ∈ ns, ∃ l ∈ c, literal.var l = n :=
 begin
-  intros c hc hsim n hn,
+  intros c hsim n hn,
   rcases exists_of_mem_map ((perm.mem_iff hsim).mpr hn) with ⟨a, ⟨ha1, ha2⟩⟩,
   use a, exact and.intro ha1 ha2
 end
@@ -123,21 +119,120 @@ begin
   exact and.intro hl2lls (and.intro (hl2n) (perm.cons l.var hl2sim))
 end
 
+theorem map_var_sim_of_var_of_mem {n : nat} {l : literal} {c : clause} : 
+  l ∈ c → l.var = n → (map var c).erase n ~ map var (c.erase l) :=
+begin
+  induction c with d ds ih,
+  { intro h, exact absurd h (not_mem_nil _) },
+  { intros hds hn,
+    by_cases l = d,
+    { rw h at hn, simp [erase_cons, h, hn] },
+    { have : l ∈ ds, from mem_of_ne_of_mem h hds,
+      have ihred := ih (mem_of_ne_of_mem h hds) hn,
+      simp [ihred, erase_cons, (ne.symm h)],
+      by_cases (d.var = l.var),
+      { simp [h, hn],
+        have : var l ∈ map var ds, from mem_map_of_mem var this,
+        rw hn at this,
+        exact perm.trans (perm_cons_erase this) (perm.cons n ihred) },
+      { simp [ne_of_ne_of_eq h hn, ihred] } } }
+end
+
 /-! ### Counting -/
 /- Counts the number of literals that evaluate to true in the clause, under some assignment -/
 def count_tt (α : assignment) (c : clause) : nat :=
-  length $ c.filter (λ l, l.eval α = tt)
+  c.countp (λ l, l.eval α = tt)
 
 /- Counts the number of literals that evaluate to false in the clause, under some assignment -/
 def count_ff (α : assignment) (c : clause) : nat :=
-  length $ c.filter (λ l, l.eval α = ff)
+  c.countp (λ l, l.eval α = ff)
 
 /- Counts the number of positive literals in the clause -/
 def count_pos (c : clause) : nat :=
-  length $ c.filter (λ l, l.is_pos)
+  c.countp (λ l, literal.is_pos l = tt)
 
 /- Counts the number of negative literals in the clause -/
 def count_neg (c : clause) : nat :=
-  length $ c.filter (λ l, literal.is_neg l)
+  c.countp (λ l, literal.is_neg l = tt)
+
+@[simp] lemma count_tt_nil (α : assignment) : count_tt α [] = 0 := by dec_trivial
+@[simp] lemma count_ff_nil (α : assignment) : count_ff α [] = 0 := by dec_trivial
+@[simp] lemma count_pos_nil : count_pos [] = 0 := by dec_trivial
+@[simp] lemma count_neg_nil : count_neg [] = 0 := by dec_trivial
+
+lemma count_tt_cons (α : assignment) (l : literal) (c : clause) : count_tt α (l :: c) = bool.to_nat (l.eval α) + count_tt α c :=
+begin
+  unfold count_tt, cases classical.em (l.eval α = tt),
+  { simp [countp_cons_of_pos (λ l, literal.eval α l = tt) c h, h, bool.to_nat, add_comm] },
+  { simp [countp_cons_of_neg (λ l, literal.eval α l = tt) c h, h, bool.to_nat, bool_eq_false h] }
+end
+
+lemma count_ff_cons (α : assignment) (l : literal) (c : clause) : count_ff α (l :: c) = bool.to_nat (!l.eval α) + count_ff α c :=
+begin
+  unfold count_ff, cases classical.em (l.eval α = ff),
+  { simp [countp_cons_of_pos (λ l, literal.eval α l = ff) c h, h, bool.to_nat, add_comm] },
+  { simp [countp_cons_of_neg (λ l, literal.eval α l = ff) c h, bool.to_nat, eq_tt_of_not_eq_ff h] }
+end
+
+lemma count_pos_cons (l : literal) (c : clause) : count_pos (l :: c) = bool.to_nat (l.is_pos) + count_pos c :=
+begin
+  unfold count_pos, cases classical.em (l.is_pos = tt),
+  { simp [countp_cons_of_pos (λ l, literal.is_pos l = tt) c h, h, bool.to_nat, add_comm] },
+  { simp [countp_cons_of_neg (λ l, literal.is_pos l = tt) c h, bool.to_nat, bool_eq_false h] }
+end
+
+lemma count_neg_cons (l : literal) (c : clause) : count_neg (l :: c) = bool.to_nat (l.is_neg) + count_neg c :=
+begin
+  unfold count_neg, cases classical.em (l.is_neg = tt),
+  { simp [countp_cons_of_pos (λ l, literal.is_neg l = tt) c h, h, bool.to_nat, add_comm] },
+  { simp [countp_cons_of_neg (λ l, literal.is_neg l = tt) c h, bool.to_nat, bool_eq_false h] }
+end
+
+lemma count_tt_singleton (α : assignment) (l : literal) : count_tt α [l] = bool.to_nat (l.eval α) := by simp [count_tt_cons α l []]
+lemma count_ff_singleton (α : assignment) (l : literal) : count_ff α [l] = bool.to_nat (!l.eval α) := by simp [count_ff_cons α l []]
+lemma count_pos_singleton (l : literal) : count_pos [l] = bool.to_nat l.is_pos := by simp [count_pos_cons l []]
+lemma count_neg_singleton (l : literal) : count_neg [l] = bool.to_nat l.is_neg := by simp [count_neg_cons l []]
+
+lemma count_pos_subset {c₁ c₂ : clause} : c₁ <+ c₂ → count_pos c₁ ≤ count_pos c₂ := 
+  assume h, by simp [count_pos, countp_le_of_sublist (λ l, literal.is_pos l = tt) h]
+
+lemma count_neg_subset {c₁ c₂ : clause} : c₁ <+ c₂ → count_neg c₁ ≤ count_neg c₂ :=
+  assume h, by simp [count_neg, countp_le_of_sublist (λ l, literal.is_neg l = tt) h]
+
+lemma exists_pos_of_odd_count_pos {c : clause} : c.count_pos.bodd → ∃ (n : nat), Pos n ∈ c :=
+begin
+  induction c with cl cls ih, --; intro h,
+  { simp [nat.bodd_zero] },
+  { intro h,
+    rcases exists_nat_of_lit cl with ⟨n, (rfl | rfl)⟩,
+    { use n, exact mem_cons_self (Pos n) cls },
+    { simp [count_pos_cons, is_pos, bool.to_nat] at h,
+      rcases ih h with ⟨n2, h2⟩, use n2, simp [h2] } }
+end
+
+-- Handling the erase case
+lemma count_pos_erase_of_mem {c : clause} {l : literal} (h : l ∈ c) : count_pos c = count_pos (c.erase l) + count_pos [l] :=
+begin
+  induction c with d ds ih,
+  { exact absurd h ( not_mem_nil _) },
+  rcases eq_or_ne_mem_of_mem h with rfl | ⟨hne, h2⟩,
+  { simp [erase_cons_head, count_pos_cons, add_comm] },
+  { rw erase_cons_tail ds (ne.symm hne),
+    have : count_pos [l] ≤ count_pos ds, from count_pos_subset (singleton_sublist.mpr h2),
+    simp [count_pos_singleton] at this,
+    simp [count_pos_cons, ih h2, add_assoc] }
+end
+
+lemma count_neg_erase_of_mem {c : clause} {l : literal} (h : l ∈ c) : count_neg c = count_neg (c.erase l) + count_neg [l] :=
+begin
+  induction c with d ds ih,
+  { exact absurd h ( not_mem_nil _) },
+  rcases eq_or_ne_mem_of_mem h with rfl | ⟨hne, h2⟩,
+  { simp [erase_cons_head, count_neg_cons, add_comm] },
+  { rw erase_cons_tail ds (ne.symm hne),
+    have : count_neg [l] ≤ count_neg ds, from count_neg_subset (singleton_sublist.mpr h2),
+    simp [count_neg_singleton] at this,
+    simp [count_neg_cons, ih h2, add_assoc] }
+end
 
 end clause
