src/cnf/cnf.lean
@@ -30,19 +30,12 @@ open list
 
 /- Instance properties -/
 instance : inhabited cnf := ⟨[default clause]⟩
-
 instance : has_mem clause cnf := ⟨list.mem⟩
-
 instance : has_emptyc cnf := ⟨list.nil⟩
-
 instance : has_union cnf := ⟨list.union⟩
-
 instance : has_inter cnf := ⟨list.inter⟩
-
 instance : has_singleton clause cnf := ⟨λ c, [c]⟩ 
-
 instance : has_insert clause cnf := ⟨list.insert⟩
-
 instance : has_append cnf := ⟨list.append⟩
 
 /-! # sim_erase -/
@@ -87,6 +80,35 @@ def eval (α : assignment) (f : cnf) : bool :=
 
 theorem eval_cons {α : assignment} {c : clause} {f : cnf} : eval α (c :: f) = (clause.eval α c && eval α f) :=
   by simp [eval, bool.band_comm]
+
+theorem eval_tt_iff_clauses_tt {α : assignment} {f : cnf} : eval α f = tt ↔ ∀ c ∈ f, clause.eval α c = tt :=
+begin
+  induction f with c cs ih,
+  { simp }, split,
+  { simp [eval_cons], 
+    intros hc hcs,
+    exact and.intro hc (ih.mp hcs) },
+  { simp [eval_cons], 
+    intros he ha,
+    simp [he, ih.mpr ha] }
+end
+
+theorem eval_ff_iff_exists_clause_ff {α : assignment} {f : cnf} : eval α f = ff ↔ ∃ c ∈ f, clause.eval α c = ff :=
+begin
+  induction f with c cs ih,
+  { simp }, split,
+  { simp [eval_cons], 
+    rintros (hc | hcs),
+    { use c, simp [hc] },
+    { rcases ih.mp hcs with ⟨c, hc1, hc2⟩,
+      use c, simp [hc1, hc2] } },
+  { 
+    simp [eval_cons],
+    split,
+    { intro hc, left, exact hc },
+    { intros a ha haf, sorry,}
+  }
+end
 
 /-
 theorem eval_double {α : assignment} {c : clause} {f : cnf} (hin : c ∈ f) : c ∈ (f.erase c) → eval α f = eval α (f.erase c) :=
@@ -146,370 +168,3 @@ def count_ff (α : assignment) (f : cnf) : nat :=
   length $ f.filter (λ c, c.eval α = ff)
 
 end cnf
-
-/- Sometimes, it is necessary to get all possible disjunctive clauses from a set of variables -/
-/- For lack of a better name, we call that operation "exploding" -/
-namespace explode
-
-open literal
-open clause
-open list
-
-/- This should ideally take in a nodup list or a finset, but lists are easier to manipulate -/
-/- Also, should ideally return a nodup list or a finset, see above comment -/
--- Here is a non-recursive definition of expl. Recursive is easier though...
-def explode_non_rec (l : list nat) : list clause :=
-  l.foldr (λ n, λ ls, (ls.map (λ e, (Pos n) :: e)) ++ (ls.map (λ e, (Neg n) :: e))) [[]]
-
-@[simp] lemma explode_non_rec_nil : explode_non_rec [] = [[]] := rfl
-
-@[simp] lemma explode_non_rec_cons {n : nat} {ns : list nat} : 
-  explode_non_rec (n :: ns) = (explode_non_rec ns).map (λ e, (Pos n) :: e) ++ (explode_non_rec ns).map (λ e, (Neg n) :: e) :=
-    by simp [explode_non_rec]
-
-/- Note: The nil case differs between the two. See if can fix above... -/
-def explode : list nat → list clause 
-  | []        := [[]]
-  | (n :: ns) := (explode ns).map (cons (Pos n)) ++ (explode ns).map (cons (Neg n))
-
--- Saying they're equal is a little dangerous - maybe saying they're similar is good enough?
-theorem explode_and_explode_rec_equiv {ns : list nat} : explode_non_rec ns = explode ns :=
-begin
-  induction ns with m ms ih,
-  { simp [explode] },
-  { simp [explode, ih] }
-end
-
-theorem length_explode : ∀ (ns : list nat), length (explode ns) = 2^(length ns)
-| []        := rfl
-| (n :: ns) := by {
-  unfold explode,
-  unfold length,
-  rw pow_succ,
-  rw two_mul,
-  rw length_append,
-  repeat {rw length_map},
-  rw length_explode ns,
-}
--- by simp [explode, length_explode ns, pow_succ, two_mul]
--- was getting replace and stack space errors, so wrote out long-hand
-
--- Corollary of the above theorem
--- Can probably be reduced in length
-theorem length_explode_pos {ns : list nat} : length (explode ns) > 0 :=
-begin
-  rw length_explode ns,
-  induction ns with d hd,
-  { unfold length, simp },
-  { unfold length,
-    rw pow_succ,
-    rw two_mul,
-    exact add_pos (ns_ih) (ns_ih)}
-end
-
--- Another corollary - is this needed?
-theorem exists_mem_of_explode : ∀ (ns : list nat), ∃ (c : clause), c ∈ explode ns :=
-  λ _, exists_mem_of_length_pos length_explode_pos
-
-theorem length_clause_explode {ns : list nat} : ∀ (c : clause), c ∈ explode ns → length c = length ns :=
-begin
-  induction ns with m ms ih,
-  { intros c h, unfold explode at h, rw (mem_singleton.mp h), refl},
-  simp only [explode, mem_cons_iff, mem_append, map_cons, mem_map],
-  rintros c (⟨c, hc, rfl⟩ | ⟨c, hc, rfl⟩);
-  { unfold length, rw ih c hc}
-end
-
-theorem mem_explode_of_mem {ns : list nat} : ∀ n ∈ ns, ∀ c ∈ explode ns, Pos n ∈ c ∨ Neg n ∈ c :=
-begin
-  induction ns with m ms ih,
-  { intros m hm, exact absurd hm (not_mem_nil _) },
-  simp only [explode, mem_cons_iff, mem_append, map_cons, mem_map],
-  rintros n (rfl | hn) c (⟨d, hd, rfl⟩ | ⟨d, hd, rfl⟩),
-  { left, apply mem_cons_self },
-  { right, apply mem_cons_self },
-  { cases ih n hn d hd with h h,
-    { left, apply mem_cons_of_mem _ h},
-    right, apply mem_cons_of_mem _ h},
-  { cases ih n hn d hd with h h,
-    { left, apply mem_cons_of_mem _ h},
-    right, apply mem_cons_of_mem _ h},
-end
-
-theorem not_mem_explode_of_not_mem {ns : list nat} : ∀ n ∉ ns, ∀ c ∈ explode ns, Pos n ∉ c ∧ Neg n ∉ c :=
-begin
-  induction ns with m ms ih,
-  { rintros m hm c hc,
-    simp [explode, hc] at hc,
-    simp [hc]},
-  simp only [explode, mem_append, map_cons, mem_map],
-  rintros p hp d hd,
-  rcases hd with ⟨c, ⟨hce, rfl⟩⟩ | ⟨c, ⟨hce, rfl⟩⟩,
-  rcases ih p (not_mem_of_not_mem_cons hp) c hce with ⟨hpos, hneg⟩,
-  { split,
-    { exact not_mem_cons_of_ne_of_not_mem (ne_pos_of_ne_nat (ne_of_not_mem_cons hp)) hpos},
-    exact not_mem_cons_of_ne_of_not_mem ne_lit_of_nat.symm hneg},
-  rcases ih p (not_mem_of_not_mem_cons hp) c hce with ⟨hpos, hneg⟩,
-  split,
-  exact not_mem_cons_of_ne_of_not_mem ne_lit_of_nat hpos,
-  exact not_mem_cons_of_ne_of_not_mem (ne_neg_of_ne_nat (ne_of_not_mem_cons hp)) hneg,
-end
-
-theorem mem_of_mem_explode {ns : list nat} : ∀ c ∈ explode ns, ∀ l ∈ c, literal.var l ∈ ns :=
-begin
-  induction ns with m ms ih,
-  { rintros c hc l hl,
-    simp [explode] at hc,
-    rw hc at hl,
-    exact absurd hl (not_mem_nil _)},
-  simp only [explode, mem_cons_iff, mem_append, map_cons, mem_map],
-  rintros c haor l hl,
-  rcases haor with ⟨a, ⟨hams, rfl⟩⟩ | ⟨a, ⟨hams, rfl⟩⟩,
-  { rcases hl with ⟨rfl, hla⟩,
-    { left, unfold var },
-    right, exact ih a hams l hl},
-  rcases hl with ⟨rfl | hlcons⟩,
-  { left, unfold var},
-  right, exact ih a hams l hl,
-end
-
--- Another way to express this is to say for all literals where it and its opposite are not in c
-theorem not_mem_of_not_mem_explode {ns : list nat} : 
-  ∀ c ∈ explode ns, ∀ (n : nat), ((Pos n ∉ c) ∧ (Neg n ∉ c)) → n ∉ ns :=
-begin
-  induction ns with m ms ih,
-  { rintros _ _ _ _, exact not_mem_nil _},
-  simp only [explode, mem_append, map_cons, mem_map],
-  rintros c (⟨a, ⟨hams, rfl⟩⟩ | ⟨a, ⟨hams, rfl⟩⟩) n ⟨hpos, hneg⟩,
-
-  apply not_mem_cons_of_ne_of_not_mem,
-  { exact ne_nat_of_ne_pos (ne_of_not_mem_cons hpos) },
-  exact ih a hams n (and.intro (not_mem_of_not_mem_cons hpos) (not_mem_of_not_mem_cons hneg)),
-
-  apply not_mem_cons_of_ne_of_not_mem,
-  { exact ne_nat_of_ne_neg (ne_of_not_mem_cons hneg) },
-  exact ih a hams n (and.intro (not_mem_of_not_mem_cons hpos) (not_mem_of_not_mem_cons hneg)),
-end
-
-theorem xor_lit_of_explode_of_nodup_list {ns : list nat} (hnodup : list.nodup ns) : ∀ n ∈ ns, ∀ c ∈ explode ns, Pos n ∉ c ∨ Neg n ∉ c :=
-begin
-  induction ns with m ms ih,
-  { rintros _ hnil _ _, exact absurd hnil (not_mem_nil n)},
-  simp only [explode, mem_append, map_cons, mem_map],
-  rintros n hn c (⟨a, ⟨hams, rfl⟩⟩ | ⟨a, ⟨hams, rfl⟩⟩),
-  { rcases eq_or_ne_mem_of_mem hn with ⟨rfl | ⟨hn1, hn2⟩⟩, -- Why do hn1 and hn2 not appear?
-    { right, apply not_mem_cons_of_ne_of_not_mem, 
-      { exact ne_lit_of_nat.symm },
-      exact (not_mem_explode_of_not_mem m (nodup_cons.mp hnodup).left a hams).right },
-    cases h with h1 h2,
-    have ihred := ih ((nodup_cons.mp hnodup).right) n h2 a hams,
-    cases ihred,
-    { left, exact not_mem_cons_of_ne_of_not_mem (ne_pos_of_ne_nat h1) ihred},
-    right, exact not_mem_cons_of_ne_of_not_mem (ne_lit_of_nat.symm) ihred},
-  { rcases eq_or_ne_mem_of_mem hn with ⟨rfl | ⟨hn1, hn2⟩⟩,
-    { left, apply not_mem_cons_of_ne_of_not_mem,
-      { exact ne_lit_of_nat },
-      exact (not_mem_explode_of_not_mem m(nodup_cons.mp hnodup).left a hams).left },
-    cases h with h1 h2,
-    have ihred := ih ((nodup_cons.mp hnodup).right) n h2 a hams,
-    cases ihred,
-    { left, exact not_mem_cons_of_ne_of_not_mem ne_lit_of_nat ihred},
-    right, exact not_mem_cons_of_ne_of_not_mem (ne_neg_of_ne_nat h1) ihred}
-end
-
-/-
-theorem aaa {ns : list nat} (hnodup : list.nodup ns) : ∀ (c : clause), ∀ n ∈ ns, xor (Pos n ∈ c) (Neg n ∈ c) → ∃ e ∈ explode ns, c.equiv e :=
-begin
-  induction ns with m ms ih,
-  { rintros _ _ hnil _, exact absurd hnil (not_mem_nil n)},
-  rintros c n hn (⟨hpos, hnneg⟩ | ⟨hneg, hnnpos⟩),
-  { cases classical.em (n = m),
-    { have : m ∉ ms, from not_mem_of_nodup_cons hnodup, 
-      rw ← h at this,
-      have exi : ∃ (cl : clause), cl ∈ explode ms, from exists_mem_of_explode ms,
-      cases exi with cl clh,
-      use (Pos n) :: cl,
-      rw h,
-      unfold explode,
-      simp,
-      split,
-      {left, use cl, exact and.intro clh rfl},
-      sorry,
-    } sorry, sorry,}
-end
-
-theorem bbb {ns : list nat} (hnodup : list.nodup ns) : ∀ (c : clause), c.length = ns.length → (∀ n ∈ ns, xor (Pos n ∈ c) (Neg n ∈ c)) → ∃ e ∈ explode ns, c.equiv e :=
-begin
-  induction ns with m ms ih,
-  { intros c h _, 
-    use ([] : clause),
-    simp [explode, length_eq_zero.mp h]},
-  { rintros c hcl hn,
-    unfold length at hcl,
-    have msnodup : ms.nodup, from nodup_of_nodup_cons hnodup,
-    have sss := hn m (mem_cons_self m ms),
-    rcases sss with ⟨hpos, hnneg⟩ | ⟨hneg, hnpos⟩,
-    have len_erase : length (c.erase (Pos m)) = length c - 1, from length_erase_of_mem hpos,
-    have : length c - 1 = (length ms + nat.succ(0)) - 1, from congr_arg nat.pred hcl,
-    rw nat.add_succ_sub_one at this,
-    rw nat.add_zero at this,
-    rw ← len_erase at this,
-    have ihred := ih msnodup (c.erase (Pos m)) this,
-    have : ∀ (n : ℕ), n ∈ ms → xor (Pos n ∈ c.erase (Pos m)) (Neg n ∈ c.erase (Pos m)),
-      { intros n hnms, have : n ∈ (m :: ms), from mem_cons_of_mem m hnms,
-        have abcd := hn n this,
-        have erasems : (m :: ms).erase m = ms, from erase_cons_head m ms,
-        rw ← erasems at hnms,
-        have nm : n ≠ m, from ((mem_erase_iff_of_nodup hnodup).mp hnms).left,
-        sorry,
-      },
-    have := ihred this,
-    cases this with e he,
-    cases he with hhe hequiv,
-    use (Pos m :: e),
-    split,
-    { unfold explode,
-      simp,
-      use e,
-      exact and.intro hhe rfl },
-    { }
-  }
-end
--/
-
-theorem perm_explode_of_perm {ns : list nat} : ∀ (l : list nat), l ~ ns → ∀ cn ∈ explode ns, ∃ cl ∈ explode l, cn ~ cl :=
-begin
-  induction ns with m ms ih,
-  { intro l, intro sim, intro cn, intro cn_sim, have : l = [], from perm.eq_nil sim, rw this,
-    unfold explode at cn_sim, have : cn = nil, from mem_singleton.mp cn_sim,
-    use ([] : clause),
-    unfold explode,
-    rw this,
-    exact and.intro (mem_singleton_self _) (perm.refl _)
-  },
-  {
-    intros l hlsim cn hcnexpl,
-    unfold explode at hcnexpl,
-    simp at hcnexpl,
-    cases hcnexpl,
-    have hlerase : l.erase m ~ (m :: ms).erase m, from perm.erase m hlsim,
-    have : (m :: ms).erase m = ms, from erase_cons_head m ms,
-    rw this at hlerase,
-    { cases hcnexpl with a ha, cases ha with ha1 ha2,
-      have ihred := ih (l.erase m) hlerase a ha1,
-      cases ihred with b hb,
-      cases hb with hb absim,
-      use (Pos m :: b),
-      sorry,
-     }, sorry,
-  }
-end
-
--- The symbol '~' means a permutation between two lists, of which clauses are, under the hood
-theorem ccc {ns : list nat} (hnodup : list.nodup ns) : ∀ (c : clause), c.length = ns.length → (∀ n ∈ ns, xor (Pos n ∈ c) (Neg n ∈ c)) → ∃ e ∈ explode ns, c ~ e :=
-begin
-  sorry,
-end
-
-theorem ddd {ns : list nat} {n : nat} : ∀ c ∈ explode (n :: ns), ∃ cn ∈ explode ns, (Pos n :: cn) ~ c ∨ (Neg n :: cn) ~ c :=
-begin
-  induction ns with m ms ih,
-  { intros c hc, use nil, unfold explode at hc, simp at hc, split, simp [explode],
-    cases hc with hcp hcn, simp [hcp], simp [hcn]},
-  simp only [explode, mem_cons_iff, mem_append, map_cons, mem_map],
-  intro c,
-  intro h,
-  cases h with h1 h2, -- h is an or
-  cases h1 with a ha, -- h1 is and exists hyp
-  cases ha with ha1 ha2,
-  cases ha1 with ha1 ha1,
-  cases ha1 with a1 ha1,
-  cases ha1 with haa1 haa2,
-  sorry,
-  sorry,
-  sorry,
-end
-
-theorem sim_erase_cons_of_explode {ns : list nat} {n : nat} (h : n ∈ ns) : ∀ c ∈ explode ns, ∃ cn ∈ explode (ns.erase n), (Pos n :: cn) ~ c ∨ (Neg n :: cn) ~ c :=
-begin
-  induction ns with m ms ih,
-  { exact absurd h (not_mem_nil _) },
-  simp only [explode, mem_cons_iff, mem_append, map_cons, mem_map],
-  intros c hc,
-  cases hc with hcp hcn,
-  { cases hcp with a ha,
-    cases ha with ha1 ha2,
-    cases classical.em (n = m),
-    { use a, simp [h_1, erase_cons_head, ha2, ha1, perm.refl] },
-    { have ihred := ih (mem_of_ne_of_mem h_1 h) a ha1,
-      cases ihred with cn hcn,
-      cases hcn with hhcn hhhcn,
-      rw erase_cons_tail ms (ne.symm h_1),
-      rw ← ha2,
-      cases hhhcn,
-      { use (Pos m :: cn), unfold explode, split,
-        { simp only [mem_cons_iff, mem_append, map_cons, mem_map],
-          left, use cn, exact and.intro hhcn (and.intro (refl _) (refl _)) },
-        left, exact perm.trans (perm.swap (Pos m) (Pos n) cn) ((perm_cons (Pos m)).mpr hhhcn) },
-      { use (Pos m :: cn), unfold explode, split,
-        { simp only [mem_cons_iff, mem_append, map_cons, mem_map],
-          left, use cn, exact and.intro hhcn (and.intro (refl _) (refl _)) },
-        right, exact perm.trans (perm.swap (Pos m) (Neg n) cn) ((perm_cons (Pos m)).mpr hhhcn) }
-    }},
-  { cases hcn with a ha,
-    cases ha with ha1 ha2,
-    cases classical.em (n = m),
-    { use a, simp [h_1, erase_cons_head, ha2, ha1, perm.refl] },
-    { have ihred := ih (mem_of_ne_of_mem h_1 h) a ha1,
-      cases ihred with cn hcn,
-      cases hcn with hhcn hhhcn,
-      rw erase_cons_tail ms (ne.symm h_1),
-      rw ← ha2,
-      cases hhhcn,
-      { use (Neg m :: cn), unfold explode, split,
-        { simp only [mem_cons_iff, mem_append, map_cons, mem_map],
-          right, use cn, exact and.intro hhcn (and.intro (refl _) (refl _)) },
-        left, exact perm.trans (perm.swap (Neg m) (Pos n) cn) ((perm_cons (Neg m)).mpr hhhcn) },
-      { use (Neg m :: cn), unfold explode, split,
-        { simp only [mem_cons_iff, mem_append, map_cons, mem_map],
-          right, use cn, exact and.intro hhcn (and.intro (refl _) (refl _)) },
-        right, exact perm.trans (perm.swap (Neg m) (Neg n) cn) ((perm_cons (Neg m)).mpr hhhcn) } } }
-end
-
-theorem explode_clause_perm_of_list {ns : list nat} : ∀ (c : clause), c ∈ explode ns → c.map var ~ ns :=
-begin 
-  induction ns with m ms ih,
-  { intros c hc, unfold explode at hc, rw (mem_singleton.mp hc), simp },
-  simp only [explode, mem_cons_iff, mem_append, map_cons, mem_map],
-  rintros c (⟨c, hc, rfl⟩ | ⟨c, hc, rfl⟩) ;
-  { simp [map, var, perm.cons m, ih c hc] }
-end
-
--- TODO cleanup with simp, etc.
-theorem explode_exhaustive {ns : list nat} : ∀ (c : clause), c.map var ~ ns → ∃ cl ∈ explode ns, c ~ cl :=
-begin
-  induction ns with m ms ih,
-  { simp [explode, perm_nil] },
-  rintros c h,
-  have : (map var c).erase m ~ (m :: ms).erase m, from perm.erase m h,
-  rw erase_cons_head m at this,
-  have hm : m ∈ map var c, from h.mem_iff.mpr (mem_cons_self m ms),
-  have : ∃ l, l ∈ c ∧ var l = m, from mem_map.mp hm,
-  cases this with l hl,
-  cases hl with hl1 hl2,
-  have testthm := erase_map_var_eq_map_var_erase m hm,
-  rcases testthm with ⟨l2, ⟨hl1, ⟨hl2, hl3⟩⟩⟩,
-  have : map var (c.erase l2) ~ ms, from (perm.symm hl3).trans this,
-  rcases ih (c.erase l2) this with ⟨cl, ⟨hclms, hclsim⟩⟩,
-  use l2 :: cl,
-  split,
-  { unfold explode, simp only [mem_cons_iff, mem_append, map_cons, mem_map], 
-    rcases pos_or_neg_of_var_eq_nat hl2 with rfl | rfl,
-    { left, use cl, exact and.intro hclms (and.intro (refl _) (refl _)) },
-    right, use cl, exact and.intro hclms (and.intro (refl _) (refl _)) },
-  have : c ~ l2 :: (c.erase l2), from perm_cons_erase hl1,
-  have onemore : l2 :: list.erase c l2 ~ l2 :: cl, from (perm_cons l2).mpr hclsim,
-  exact perm.trans this onemore
-end
-
-end explode
