src/xor/xor.lean
@@ -9,47 +9,170 @@
 -/
 
 import data.bool
-import cayden.cnf
+import data.list.basic
+
+import cnf.literal
+import cnf.clause
+import cnf.cnf
+import cnf.explode
 import basic
 
-/- Let's define an XOR gate -/
-def xor_g := list literal
+/- An n-literal XOR gate is a list of those literals -/
+def xor_gate := list literal
 
-namespace xor_g
+namespace xor_gate
 
+open list
 open literal
+open clause
+open cnf
+open explode
 
 /- Evaluates the XOR gate under an assignment -/
-def eval (α : assignment) (g : xor_g) : bool :=
-  g.foldr (λ l, λ b, b ⊕ l.eval α) ff
+def eval (α : assignment) (g : xor_gate) : bool :=
+  g.foldr (λ l b, b ⊕ l.eval α) ff
 
-def to_cnf : xor_g → cnf
-  | []        := []
-  | [l]       := [[l]]
-  | (l :: ls) := list.map (λ r, let (c, p) := r in cond p (l.set_pos :: c) (l.set_neg :: c))) (explode.expl_parity (ls.map (λ x, x.var)))
+@[simp] lemma eval_nil (α : assignment) : eval α [] = ff := rfl
 
-def evaluate_xor_helper (α : literal → bool) : list literal → nat → nat
-  | [] n        := n
-  | (l :: ls) n := bool.to_nat (α l) + evaluate_xor_helper ls n
+lemma eval_cons (α : assignment) (l : literal) (g : xor_gate) : eval α (l :: g) = bxor (literal.eval α l) (eval α g) :=
+  by simp [eval, foldr_cons, bool.bxor_comm]
 
-def explode_with_negated_count : list literal → list (list literal × nat)
-  | []        := [([], 0)]
-  | (l :: ls) :=
-    let
-      e : list (list literal × nat) := explode_with_negated_count ls,
-      l1 := list.map (λx, let (lss, c) := x in prod.mk (literal.Pos (nat_from_literal l) :: lss) (c : nat)) e,
-      l2 := list.map (λx, let (lss, c) := x in prod.mk (literal.Neg (nat_from_literal l) :: lss) (c + 1)) e
-    in
-      list.append l1 l2
+theorem eval_cons_conjunctive (α : assignment) (l : literal) (g : xor_gate) : 
+  eval α (l :: g) = (literal.eval α l || eval α g) && (!(literal.eval α l) || !(eval α g)) :=
+by simp only [← bxor_conjunctive, eval_cons α l g]
 
-def xor_to_cnf : list literal → list (list literal)
-  | []        := [[]]
-  | [l]       := [[l]]
-  | (l :: ls) := 
-    let
-      ls_ex := explode_with_negated_count ls
-    in
-      list.map (λx, let (lss, (c : nat)) := x in 
-        cond (c % 2 = 0) (literal.Pos (nat_from_literal l) :: lss) (literal.Neg (nat_from_literal l) :: lss)) ls_ex
+theorem eval_cons_disjunctive (α : assignment) (l : literal) (g : xor_gate) :
+  eval α (l :: g) = (!(literal.eval α l) && eval α g) || (literal.eval α l && !(eval α g)) :=
+by simp only [← bxor_disjunctive, eval_cons α l g]
 
-end xor_g
+/- Using a recursive evaluation function is sometimes more convenient -/
+def eval_rec (α : assignment) : xor_gate → bool
+| []        := ff
+| (l :: ls) := l.eval α ⊕ eval_rec ls
+
+/- To use the recursive definition, we need to prove that the two functions are equivalent -/
+theorem eval_and_eval_rec_equiv {α : assignment} {g : xor_gate} : eval α g = eval_rec α g :=
+begin
+  induction g with l ls ih,
+  { simp [eval_rec, eval] },
+  { simp [eval_rec, ih, eval_cons] },
+end
+
+/- The XOR gate evaluates to true if an odd number of literals evaluates to true -/
+theorem xor_odd_eval_tt {α : assignment} {g : xor_gate} : g.eval α = nat.bodd (g.countp (λ l, l.eval α = tt)) :=
+begin
+  induction g with l ls ih,
+  split; { simp [eval] },
+  by_cases (l.eval α = tt),
+  { simp [h, ih, eval_cons] },
+  { simp at h, simp [h, ih, eval_cons] }
+end
+
+-- Let's start easier: turning a list of natural numbers into a cnf form
+-- We use explode.explode, which takes in a list of nats. Alternatively, we take a list of ints and get tricky with negatives meaning flipped
+-- Note the return value of explode is list clause, which is cnf
+def nat_to_xor_cnf : list nat → cnf
+| []        := [[]]
+| (n :: ns) := (explode ns).map (λ c, cond (nat.bodd c.count_neg = ff) ((Pos n) :: c) ((Neg n) :: c))
+
+theorem nat_to_xor_cnf_length {ns : list nat} : ns ≠ [] → length (nat_to_xor_cnf ns) = 2^(length ns - 1) :=
+begin
+  cases classical.em (ns = nil); intro hns,
+  { exact absurd h hns },
+  { rcases exists_cons_of_ne_nil hns with ⟨w, ⟨l, rfl⟩⟩, 
+    simp only [nat_to_xor_cnf, length_map, length_cons, length_explode, nat.succ_sub_one] }
+end
+
+theorem map_var_sim_of_mem_nat_to_xor : ∀ (ns : list nat), ∀ (c : clause), c ∈ nat_to_xor_cnf ns → c.map var ~ ns
+| []        := by { simp [nat_to_xor_cnf] }
+| (n :: ns) := begin
+  simp only [nat_to_xor_cnf, mem_map, mem_append],
+  rintros c ⟨a, ⟨ha1, ha2⟩⟩,
+  by_cases a.count_neg.bodd = tt,
+  { simp [h] at ha2, simp [← ha2, var, map_var_sim_of_mem_explode a ha1] },
+  { simp [bool_eq_false h] at ha2, simp [← ha2, var, map_var_sim_of_mem_explode a ha1] }
+end
+
+theorem exists_mem_explode_sim_of_mem_nat_to_xor {ns : list nat} : 
+  ∀ (c : clause), c ∈ nat_to_xor_cnf ns → ∃ cl ∈ explode ns, c ~ cl :=
+assume c h, mem_explode_sim_of_map_var_sim c (map_var_sim_of_mem_nat_to_xor ns c h)
+
+-- Riskier, but what else can you do?
+theorem exists_mem_explode_of_mem_nat_to_xor :
+  ∀ (ns : list nat), ∀ (c : clause), c ∈ nat_to_xor_cnf ns → c ∈ explode ns
+| []        := by simp [nat_to_xor_cnf]
+| (n :: ns) := begin
+  simp [nat_to_xor_cnf, mem_map, mem_append],
+  intros c hc,
+  by_cases c.count_neg.bodd = tt,
+  { simp [h], have : (Pos n).var = n, simp [var],
+    exact mem_explode_cons_of_lit c hc this },
+  { simp [bool_eq_false h], have : (Neg n).var = n, simp [var],
+    exact mem_explode_cons_of_lit c hc this }
+end
+
+-- Technically not a proof by induction, fix later?
+theorem nat_to_xor_cnf_contains_all_even_negated_clauses {ns : list nat} :
+  ∀ {c : clause}, c.map var = ns → (nat.bodd c.count_neg = ff) → c ∈ nat_to_xor_cnf ns :=
+begin
+  induction ns with m ms ih,
+  { simp [nat_to_xor_cnf] },
+  { intros c hc,
+  rcases exists_cons_of_map_cons hc with ⟨l, ls, rfl, hl, hls⟩,
+  rcases pos_or_neg_of_var_eq_nat hl with rfl | rfl;
+  { simp [count_neg_cons, is_neg, bool.to_nat, nat_to_xor_cnf],
+    intro hcount, use ls,
+    simp [hcount, mem_explode_of_map_var_eq hls] } }
+end
+
+-- TODO cleanup
+theorem nat_to_xor_cnf_contains_no_even_negated_clauses {ns : list nat} (hns: ns ≠ []) :
+  ∀ {c : clause}, c.map var = ns → (nat.bodd c.count_neg = tt) → c ∉ nat_to_xor_cnf ns :=
+begin
+  induction ns with m ms ih,
+  { contradiction },
+  {
+    intros c hc,
+    rcases exists_cons_of_map_cons hc with ⟨l, ls, rfl, hl, hls⟩,
+    rcases pos_or_neg_of_var_eq_nat hl with rfl | rfl,
+    { simp [count_neg_cons, is_neg, bool.to_nat, nat_to_xor_cnf],
+      intros hcount x hx,
+      by_cases (count_neg x).bodd = tt,
+      { simp [h], intro h2,
+        exact absurd (head_eq_of_cons_eq h2) ne_pos_neg_of_nat.symm },
+      { simp [bool_eq_false h], -- Lots of fooling around with ¬ and ff, clean up
+        intro h2, have h2 := tail_eq_of_cons_eq h2,
+        rw h2 at h,
+        rw hcount at h,
+        exact absurd (refl tt) h } },
+    { simp [count_neg_cons, is_neg, bool.to_nat, nat_to_xor_cnf],
+      intros hcount x hx,
+      by_cases (count_neg x).bodd = tt,
+      { simp [h], intro h2,
+        have h2 := tail_eq_of_cons_eq h2,
+        rw h2 at h,
+        exact bool_iff_false.mpr hcount h },
+      { simp [bool_eq_false h], intro h2,
+        exact absurd (head_eq_of_cons_eq h2) ne_pos_neg_of_nat } } }
+end
+
+-- We prove that the naive encoding is equivalent to an XOR gate of all positive literals
+theorem nat_to_xor_cnf_correct {α : assignment} : ∀ (ns : list nat), cnf.eval α (nat_to_xor_cnf ns) = eval α (ns.map Pos)
+| []        := by simp [nat_to_xor_cnf]
+| (n :: ns) := begin
+  --simp [nat_to_xor_cnf, map_cons, eval_cons],
+  by_cases ((map Pos (n :: ns)).countp (λ l, literal.eval α l = tt)).bodd = tt,
+  { --  We are in the odd case, meaning that we should satisfy
+    have : eval α (map Pos (n :: ns)) = ((map Pos (n :: ns)).countp (λ l, literal.eval α l = tt)).bodd, from xor_odd_eval_tt,
+    rw this.symm at h,
+    rw h,
+    simp [nat_to_xor_cnf],
+    sorry,
+
+
+  }
+  sorry,
+  sorry,
+end
+
+end xor_gate
