src/basic.lean
@@ -8,6 +8,7 @@
 -/
 
 import data.bool
+import data.list.basic
 
 -- Define shorthand for XOR
 notation a ⊕ b := bxor a b
@@ -34,3 +35,14 @@ theorem bxor_disjunctive : ∀ (a b : bool), bxor a b = (!a && b) || (a && !b)
 | tt ff := dec_trivial
 | ff tt := dec_trivial
 | ff ff := dec_trivial
+
+-- Some facts about map that help
+theorem exists_cons_of_map_cons {α β : Type} {f : α → β} {b : β} {bs : list β} :
+  ∀ {l : list α}, list.map f l = b :: bs → ∃ h L, l = h :: L ∧ f h = b ∧ list.map f L = bs
+| [] := by { contradiction }
+| (x :: xs) := begin 
+  simp [list.map_cons],
+  intros hx hxs, split,
+  { use x, exact hx},
+  { use xs, exact hxs}
+end
